Define and prove the soundness of the update transforms of the bitmap index

fiat2/src/fiat2/BitmapIndex.v
@@ -25,7 +25,7 @@ Section WithHole.
     EFold (EVar hole) (ERecord [("0", EAtom (AInt 0)); ("1", EAtom (ANil (Some TInt))); ("2", EAtom (AEmptyDict None))])
       tup acc
       (ERecord [("0", EBinop OPlus n (EAtom (AInt 1))); ("1", EBinop OCons n l); ("2", ETernop OInsert d n (EVar tup))]).
-*)
+   *)
   Definition is_pk_tbl_ty (t : type) : bool :=
     match t with
     | TList _ => true
@@ -96,25 +96,25 @@ Section WithHole.
                       | _ => VUnit
                       end (VInt 1));
                   ("1",
-             match
-               match acc0
-               with
-               | VRecord l => record_proj "1" l
-               | _ => VUnit
-               end
-             with
-             | VDict d =>
-                 VDict
-                   (dict_insert
+                    match
                       match acc0
                       with
-                      | VRecord l => record_proj "0" l
+                      | VRecord l => record_proj "1" l
                       | _ => VUnit
-                      end v d)
-             | _ => VUnit
-             end)]) (VRecord [("0", VInt 0); ("1", VDict [])])
-        l1
-  | _ => VUnit
+                      end
+                    with
+                    | VDict d =>
+                        VDict
+                          (dict_insert
+                             match acc0
+                             with
+                             | VRecord l => record_proj "0" l
+                             | _ => VUnit
+                             end v d)
+                    | _ => VUnit
+                    end)]) (VRecord [("0", VInt 0); ("1", VDict [])])
+            l1
+      | _ => VUnit
       end.
 
     Lemma fiat2_gallina_to_pk_idx : forall tbl_v, interp_expr (word:=word) map.empty (map.put map.empty hole tbl_v) to_pk_idx = gallina_to_pk_idx tbl_v.
@@ -141,9 +141,9 @@ Section WithHole.
       end.
 
     Lemma map_fst_flat_map2 : forall A B l l',
-      incl (List.map fst
-              (flat_map2 (fun (k:A) (v:B) => [(k, v)]) l l'))
-        l.
+        incl (List.map fst
+                (flat_map2 (fun (k:A) (v:B) => [(k, v)]) l l'))
+          l.
     Proof.
       induction l; intros.
       1: apply incl_nil_l.
@@ -325,6 +325,10 @@ Section WithHole.
           1: apply StronglySorted_dict_sort. }
     Qed.
 
+    Instance pk_idx : IndexInterface2.index := IndexInterface2.mk hole to_pk_idx pk_idx_ty is_pk_tbl_ty.
+
+    Instance pk_idx_ok : IndexInterface2.ok pk_idx pk_idx_wf :=
+      IndexInterface2.Build_ok pk_idx pk_idx_wf pk_idx_ty_wf to_pk_idx_ty to_pk_idx_wf.
   End WithMap.
 End WithHole.
 
@@ -411,53 +415,243 @@ Section WithHole.
       repeat f_equal. rewrite_map_get_put_goal.
       reflexivity.
     Qed.
+
+    Instance bitmap : IndexInterface2.index := IndexInterface2.mk hole to_bitmap bitmap_ty is_bitmap_tbl_ty.
+
+    Instance bitmap_ok : IndexInterface2.ok bitmap bitmap_wf :=
+      IndexInterface2.Build_ok bitmap bitmap_wf bitmap_ty_wf to_bitmap_ty to_bitmap_wf.
   End WithMap.
 End WithHole.
 
 Section WithTags.
   Context (id_tag aux_tag pk_idx_tag bm_tag : string).
 
-  Section filter_to_bitmap_lookup.
-    Context (tbl attr str : string).
-    Context (x1 b acc : string).
-    Context (H_NoDup : is_NoDup_opaque [x1; b; acc]).
+  Context (pk_hole pk_tup pk_acc : string).
+  Context (H_NoDup_pk : is_NoDup_opaque [pk_tup; pk_acc]).
 
-    Definition use_bitmap bm d :=
-      let n := EAccess (EVar acc) "0" in
-      let l := EAccess (EVar acc) "1" in
-      EFold bm (ERecord [("0", EAtom (AInt 0)); ("1", EAtom (ANil None))])
-        b acc (ERecord [("0", EBinop OPlus n (EAtom (AInt 1)));
-                        ("1", EIf (EVar b)
-                                (EOptMatch (EBinop OLookup d n)
-                                   l x1 (EBinop OCons (EVar x1) l))
-                                l)]).
+  Notation pk_idx_wf := (pk_idx_wf pk_hole pk_tup pk_acc).
 
-    Definition filter_to_bitmap_lookup_head (e : expr) :=
-      match e with
-      | EFilter LikeList (EAccess (ELoc tbl0) (id_tag0)) x
-          (EBinop OEq (EAccess (EVar x0) attr0) (EAtom (AString str0))) =>
-          if (all_eqb [(tbl, [tbl0]); (attr, [attr0]); (x, [x0; x1]); (id_tag, [id_tag0]); (str, [str0])])
-          then
-            let n := EAccess (EVar acc) "0" in
-            let l := EAccess (EVar acc) "1" in
-            EAccess
-              (use_bitmap
-                 (EAccess (EAccess (ELoc tbl) aux_tag) bm_tag)
-                 (EAccess (EAccess (EAccess (ELoc tbl) aux_tag) pk_idx_tag) "1"))
-              "1"
-          else e
-      | _ => e
-      end.
+  Context (attr str : string).
+  Context (bm_hole : string).
+  Context (bm_tup : string).
 
-    Section WithMap.
-      Context {tenv : map.map string type} {tenv_ok : map.ok tenv}.
-      Context {width: Z} {word: word.word width} {word_ok: word.ok word}.
-      Notation value := (value (width:=width)).
-      Context {locals : map.map string value} {locals_ok : map.ok locals}.
+  Notation is_bitmap_tbl_ty := (is_bitmap_tbl_ty attr).
+  Notation bitmap_wf := (bitmap_wf attr str bm_hole bm_tup).
+
+  Section WithMap.
+    Context {tenv : map.map string type} {tenv_ok : map.ok tenv}.
+    Context {width: Z} {word: word.word width} {word_ok: word.ok word}.
+    Notation value := (value (width:=width)).
+    Context {locals : map.map string value} {locals_ok : map.ok locals}.
+
+
+    Section cons_to_pk_idx_update.
+      Context (y : string).
+
+      Notation eto_pk_idx tup0 tup1 acc0 acc1 acc2 acc3 e :=
+        (EFold e (ERecord [("0", EAtom (AInt 0)); ("1", EAtom (AEmptyDict None))])
+           tup0 acc0
+           (ERecord [("0", EBinop OPlus (EAccess (EVar acc1) "0") (EAtom (AInt 1))); ("1", ETernop OInsert (EAccess (EVar acc2) "1") (EAccess (EVar acc3) "0") (EVar tup1))])).
+
+      Definition cons_to_pk_idx_update_head (e : expr) :=
+        match e with
+        | eto_pk_idx tup0 tup1 acc0 acc1 acc2 acc3 (EBinop OCons e1 e2) =>
+            if (all_eqb [(tup0, [tup1]); (acc0, [acc1; acc2; acc3])] && (negb (String.eqb tup0 acc0)) &&
+                 negb (free_immut_in y e1))%bool
+            then ELet (eto_pk_idx tup0 tup0 acc0 acc0 acc0 acc0 e2) y
+                      (ERecord [("0", EBinop OPlus (EAccess (EVar y) "0") (EAtom (AInt 1))); ("1", ETernop OInsert (EAccess (EVar y) "1") (EAccess (EVar y) "0") e1)])
+            else e
+        | _ => e
+        end.
+
+      (* ??? move *)
+      Lemma not_free_immut_put_ty2 : forall (x : string) (e : expr) (Gstore Genv : tenv) (t t' : type),
+          free_immut_in x e = false ->
+          type_of Gstore Genv e t ->
+          type_of Gstore (map.put Genv x t') e t.
+      Proof.
+        intros. destruct (map.get Genv x) eqn:E.
+        1:{ rewrite <- Properties.map.put_remove_same.
+            eapply type_of_strengthen;
+              [
+              | apply map_incl_refl
+              | apply map_incl_step_r; try apply map_incl_refl;
+                apply map.get_remove_same ].
+            eapply not_free_immut_put_ty; eauto.
+            rewrite Properties.map.put_remove_same, Properties.map.put_noop; eauto. }
+        1:{ eapply type_of_strengthen; eauto using map_incl_refl.
+            apply map_incl_step_r; auto using map_incl_refl. }
+      Qed.
+
+      Lemma cons_to_pk_idx_update_head_preserve_ty : forall (Gstore : tenv),
+              preserve_ty Gstore cons_to_pk_idx_update_head.
+      Proof.
+        unfold preserve_ty; intros. repeat destruct_subexpr.
+        cbn. repeat (case_match; auto).
+        rewrite !Bool.andb_true_iff, !Bool.negb_true_iff in *; intuition auto.
+        rewrite eqb_eq, eqb_neq in *; subst. repeat invert_type_of_clear.
+        repeat rewrite_map_get_put_hyp.
+        repeat (try clear_refl; repeat do_injection).
+        repeat invert_type_of_op_clear.
+        repeat (destruct tl; cbn in *; try discriminate).
+        repeat (destruct tl0; cbn in *; try discriminate).
+        destruct p, p0, p1, p2; cbn in *. repeat (invert_cons; clear_refl).
+        lazymatch goal with
+          H: Permutation [_; _] _ |- _ =>
+            apply Permutation_length_2_inv in H end; destruct_or; subst.
+        2:{ invert_SSorted. invert_Forall. discriminate. }
+         lazymatch goal with
+          H: Permutation [_; _] _ |- _ =>
+            apply Permutation_length_2 in H end; intuition idtac; try discriminate.
+        repeat invert_pair. repeat invert_Forall2.
+        repeat invert_type_of_clear; invert_type_of_op_clear.
+        repeat rewrite_map_get_put_hyp. repeat (do_injection; clear_refl).
+        cbn in *. repeat (clear_refl; do_injection). invert_type_of_op_clear.
+        do 2 econstructor; eauto; cbn; auto.
+        1:{ instantiate(1:=TRecord [("0", TInt); ("1", TDict TInt t5)]).
+            repeat (econstructor; eauto). }
+        all: repeat (econstructor; eauto); repeat rewrite_map_get_put_goal; eauto.
+        apply not_free_immut_put_ty2; auto.
+      Qed.
+
+      Lemma fold_to_pk_idx : forall store (env : locals) tup acc e,
+          tup <> acc ->
+          interp_expr store env (eto_pk_idx tup tup acc acc acc acc e) =
+            gallina_to_pk_idx (interp_expr store env e).
+      Proof.
+        intros. cbn.
+        unfold gallina_to_pk_idx.
+        case_match; auto.
+        apply In_fold_right_ext with (P:=fun _ => True); intuition idtac.
+        repeat f_equal; unfold get_local;
+          repeat rewrite_map_get_put_goal; auto; use_is_NoDup.
+      Qed.
+
+      Lemma cons_to_pk_idx_update_head_preserve_sem : forall (Gstore : tenv) (store : locals),
+          preserve_sem Gstore store cons_to_pk_idx_update_head.
+      Proof.
+        unfold preserve_sem; intros. repeat destruct_subexpr.
+        cbn [cons_to_pk_idx_update_head]. repeat (case_match; auto; []).
+        cbn in * |-.
+        rewrite !Bool.andb_true_iff, !Bool.negb_true_iff in *; intuition idtac.
+        rewrite eqb_eq, eqb_neq in *; subst. repeat invert_type_of_clear.
+        repeat rewrite_map_get_put_hyp.
+        repeat (try clear_refl; repeat do_injection).
+        repeat invert_type_of_op_clear.
+        enough (E_Let: forall e1 e2 x, interp_expr store env (ELet e1 x e2) = interp_expr store (map.put env x (interp_expr store env e1)) e2); auto.
+        rewrite E_Let.
+        repeat rewrite fold_to_pk_idx; auto.
+        cbn. apply_type_sound e1_2. invert_type_of_value_clear.
+        unfold gallina_to_pk_idx. cbn. repeat f_equal.
+        1:{ unfold get_local; rewrite_map_get_put_goal. reflexivity. }
+        1:{ unfold get_local; rewrite_map_get_put_goal.
+            repeat (case_match; auto; []). do 2 f_equal.
+            symmetry; eapply not_free_immut_put_sem; eauto. }
+      Qed.
+
+      Lemma cons_to_pk_idx_update_head_sound :
+        expr_transf_sound (locals:=locals) cons_to_pk_idx_update_head.
+      Proof.
+        unfold expr_transf_sound; intros.
+        intuition idtac.
+        1: eapply cons_to_pk_idx_update_head_preserve_ty; eauto.
+        1: eapply cons_to_pk_idx_update_head_preserve_sem; [ | | eauto .. ]; auto.
+      Qed.
+    End cons_to_pk_idx_update.
+
+    Section cons_to_bitmap_update.
+      Definition cons_to_bitmap_update_head (e : expr) :=
+        match e with
+        | EFlatmap LikeList (EBinop OCons e1 e2) tup0
+           (EBinop OCons
+              (EBinop OEq (EAccess (EVar tup1) attr) (EAtom (AString str)))
+              (EAtom (ANil (Some TBool)))) =>
+            if all_eqb [(tup0, [tup1])]
+            then EBinop OCons
+                   (EBinop OEq (EAccess e1 attr) (EAtom (AString str)))
+                   (EFlatmap LikeList e2 tup0
+                      (EBinop OCons
+                         (EBinop OEq (EAccess (EVar tup1) attr) (EAtom (AString str)))
+              (EAtom (ANil (Some TBool)))))
+            else e
+        | _ => e
+        end.
+
+      Lemma cons_to_bitmap_update_head_preserve_ty : forall (Gstore : tenv),
+              preserve_ty Gstore cons_to_bitmap_update_head.
+      Proof.
+        unfold preserve_ty; intros. repeat destruct_subexpr.
+        cbn. repeat (case_match; auto).
+        rewrite !Bool.andb_true_iff in *; intuition auto.
+        rewrite eqb_eq in *; subst. repeat invert_type_of_clear.
+        repeat rewrite_map_get_put_hyp. do_injection.
+        repeat invert_type_of_op_clear.
+        repeat invert_type_of_atom.
+        repeat (econstructor; eauto).
+        rewrite_map_get_put_goal. reflexivity.
+      Qed.
+
+      Lemma cons_to_bitmap_update_head_preserve_sem : forall (Gstore : tenv) (store : locals),
+          preserve_sem Gstore store cons_to_bitmap_update_head.
+      Proof.
+        unfold preserve_sem; intros. repeat destruct_subexpr.
+        cbn [cons_to_bitmap_update_head]. repeat (case_match; auto; []).
+        cbn in * |-.
+        rewrite !Bool.andb_true_iff in *; intuition idtac.
+        rewrite eqb_eq in *; subst. repeat invert_type_of_clear.
+        repeat rewrite_map_get_put_hyp.
+        repeat (try clear_refl; repeat do_injection).
+        repeat invert_type_of_op_clear.
+        cbn. case_match; auto. f_equal.
+        cbn. repeat f_equal. unfold get_local; rewrite_map_get_put_goal.
+        reflexivity.
+      Qed.
+
+      Lemma cons_to_bitmap_update_head_sound :
+        expr_transf_sound (locals:=locals) cons_to_bitmap_update_head.
+      Proof.
+        unfold expr_transf_sound; intros.
+        intuition idtac.
+        1: eapply cons_to_bitmap_update_head_preserve_ty; eauto.
+        1: eapply cons_to_bitmap_update_head_preserve_sem; [ | | eauto .. ]; auto.
+      Qed.
+    End cons_to_bitmap_update.
+
+    Section filter_to_bitmap_lookup.
+      Context (x b acc : string).
+      Context (H_NoDup : is_NoDup_opaque [x; b; acc]).
+      Context (tbl : string).
+
+      Definition use_bitmap bm d :=
+        let n := EAccess (EVar acc) "0" in
+        let l := EAccess (EVar acc) "1" in
+        EFold bm (ERecord [("0", EAtom (AInt 0)); ("1", EAtom (ANil None))])
+          b acc (ERecord [("0", EBinop OPlus n (EAtom (AInt 1)));
+                          ("1", EIf (EVar b)
+                                  (EOptMatch (EBinop OLookup d n)
+                                     l x (EBinop OCons (EVar x) l))
+                                  l)]).
+
+      Definition filter_to_bitmap_lookup_head (e : expr) :=
+        match e with
+        | EFilter LikeList (EAccess (ELoc tbl0) (id_tag0)) x
+            (EBinop OEq (EAccess (EVar x0) attr0) (EAtom (AString str0))) =>
+            if (all_eqb [(tbl, [tbl0]); (attr, [attr0]); (x, [x0; x]); (id_tag, [id_tag0]); (str, [str0])])
+            then
+              let n := EAccess (EVar acc) "0" in
+              let l := EAccess (EVar acc) "1" in
+              EAccess
+                (use_bitmap
+                   (EAccess (EAccess (ELoc tbl) aux_tag) bm_tag)
+                   (EAccess (EAccess (EAccess (ELoc tbl) aux_tag) pk_idx_tag) "1"))
+                "1"
+            else e
+        | _ => e
+        end.
 
       Lemma filter_to_bitmap_lookup_head_preserve_ty : forall tl t aux_tl (Gstore : tenv),
           type_wf t -> is_pk_tbl_ty t = true ->
-          is_bitmap_tbl_ty attr t = true ->
+          is_bitmap_tbl_ty t = true ->
           map.get Gstore tbl = Some (TRecord tl) ->
           access_record tl id_tag = Success t ->
           access_record tl aux_tag = Success (TRecord aux_tl) ->
@@ -491,10 +685,18 @@ Section WithTags.
         cbn; reflexivity.
       Qed.
 
-      Context (pk_hole pk_tup pk_acc : string).
-      Context (H_NoDup_pk : is_NoDup_opaque [pk_tup; pk_acc]).
-
-      Notation pk_idx_wf := (pk_idx_wf pk_hole pk_tup pk_acc).
+      Definition aux_ty_for_idx idx_tag idx_ty (aux_ty : type -> type) : Prop :=
+        forall t,
+          match aux_ty t with
+          | TRecord tl =>
+              access_record tl id_tag = Success t /\
+                match access_record tl aux_tag with
+                | Success (TRecord aux_tl) =>
+                    access_record aux_tl idx_tag = Success (idx_ty t)
+                | _ => False
+                end
+          | _ => False
+          end.
 
       Definition aux_wf_for_idx idx_tag idx_wf (v : value) : Prop :=
         match v with
@@ -508,16 +710,12 @@ Section WithTags.
                         idx_wf v_id v_idx
                     | _ => False
                     end
-              | _ => False
-              end
-          | _ => False
-          end
+                | _ => False
+                end
+            | _ => False
+            end
         | _ => False
         end.
-
-      Context (bm_hole : string).
-      Context (bm_tup : string).
-      Notation bitmap_wf := (bitmap_wf attr str bm_hole bm_tup).
 
       (* ??? TODO: move *)
       Lemma Forall2_access_record : forall A A' P l l' x (a : A) (a' : A'),
@@ -668,8 +866,8 @@ Section WithTags.
         cbn [flat_map2 Datatypes.length mk_ids app].
         constructor;
           (assert (Heq: forall (k v : value) l l',
-                (k, v) :: flat_map2 (fun k v => [(k, v)]) l l' = flat_map2 (fun k v => [(k, v)]) (k :: l) (v :: l')); [ reflexivity | ];
-          assert (Heq': VInt (Z.of_nat (Datatypes.length l)) :: mk_ids (width:=width) (Datatypes.length l) = mk_ids (Datatypes.length (a :: l)));  [ reflexivity | ]).
+                 (k, v) :: flat_map2 (fun k v => [(k, v)]) l l' = flat_map2 (fun k v => [(k, v)]) (k :: l) (v :: l')); [ reflexivity | ];
+           assert (Heq': VInt (Z.of_nat (Datatypes.length l)) :: mk_ids (width:=width) (Datatypes.length l) = mk_ids (Datatypes.length (a :: l)));  [ reflexivity | ]).
         1:{ apply In_dict_lookup; auto using StronglySorted_dict_sort.
             1:{ eapply Permutation_NoDup.
                 1: eapply Permutation_map, Permuted_dict_sort.
@@ -742,9 +940,9 @@ Section WithTags.
         1:{ apply access_record_sound in H4.
             apply in_map with (f:=fst) in H4; cbn in H4.
             lazymatch goal with
-                H: Forall2 (fun _ _ => _ /\ _) _ _ |- _ =>
-                  apply Forall2_split in H
-              end; intuition idtac.
+              H: Forall2 (fun _ _ => _ /\ _) _ _ |- _ =>
+                apply Forall2_split in H
+            end; intuition idtac.
             apply Forall2_fst_eq in H2.
             rewrite <- H2 in H4.
             apply In_access_record in H4; destruct_exists.
@@ -756,7 +954,7 @@ Section WithTags.
 
       Lemma filter_to_bitmap_lookup_head_preserve_sem : forall (Gstore : tenv) (store : locals) tl t aux_tl,
           type_wf t -> is_pk_tbl_ty t = true ->
-          is_bitmap_tbl_ty attr t = true ->
+          is_bitmap_tbl_ty t = true ->
           map.get Gstore tbl = Some (TRecord tl) ->
           access_record tl id_tag = Success t ->
           access_record tl aux_tag = Success (TRecord aux_tl) ->
@@ -812,195 +1010,43 @@ Section WithTags.
         end.
         destruct_exists; rewrite_l_to_r. reflexivity.
       Qed.
-    End WithMap.
+    End filter_to_bitmap_lookup.
 
-  End filter_to_bitmap_lookup.
+    Context (x b acc : string).
+    Context (H_NoDup : is_NoDup_opaque [x; b; acc]).
 
-End WithTags.
+    Ltac invert_tenv_wf_with_globals :=
+      lazymatch goal with H: tenv_wf_with_globals _ _ _ |- _ => inversion H; subst end.
 
-(*
-    Context (tbl attr1 str1 attr2 str2 : string).
-    Context (x1 x2 b acc : string).
-    Context (H_NoDup : is_NoDup_opaque [x1; x2; b; acc]).
-
-    Definition and_bitmaps bm1 bm2 :=
-      EFlatmap2 bm1 bm2
-        x1 x2 (EBinop OCons (EBinop OAnd (EVar x1) (EVar x2)) (EAtom (ANil None))).
-
-    Definition use_bitmap bm d :=
-      let n := EAccess (EVar acc) "0" in
-      let l := EAccess (EVar acc) "1" in
-      EFold bm (ERecord [("0", EAtom (AInt 0)); ("1", EAtom (ANil None))])
-        b acc (ERecord [("0", EBinop OPlus n (EAtom (AInt 1)));
-                        ("1", EIf (EVar b)
-                                (EOptMatch (EBinop OLookup d n)
-                                   l x1 (EBinop OCons (EVar x1) l))
-                                l)]).
-
-    Definition and_filter_to_lookup_head (e : expr) :=
-      match e with
-      | EFilter LikeList (EAccess (ELoc tbl0) (id_tag0)) x
-          (EBinop OAnd (EBinop OEq (EAccess (EVar x0) attr1') str1')
-             (EBinop OEq (EAccess (EVar x1) attr2') str2')) =>
-          if (all_eqb [(tbl, [tbl0]); (attr1, [attr1']); (attr2, [attr2']); (x, [x0; x1]); (id_tag, [id_tag0])])
-          then
-            let n := EAccess (EVar acc) "0" in
-            let l := EAccess (EVar acc) "1" in
-            EAccess
-              (use_bitmap
-                 (and_bitmaps
-                    (EAccess (EAccess (ELoc tbl) aux_tag) bm1_tag)
-                    (EAccess (EAccess (ELoc tbl) aux_tag) bm2_tag))
-                 (EAccess (EAccess (EAccess (ELoc tbl) aux_tag) pk_idx_tag) "1"))
-              "1"
-          else e
-      | _ => e
-      end.
-
-  Section WithMap.
-    Context {tenv : map.map string type} {tenv_ok : map.ok tenv}.
-    Context {width: Z} {word: word.word width} {word_ok: word.ok word}.
-    Notation value := (value (width:=width)).
-    Context {locals : map.map string value} {locals_ok : map.ok locals}.
-
-    Lemma and_bitmaps_ty : forall Gstore Genv e1 e2,
-        type_of Gstore Genv e1 (TList TBool) ->
-        type_of Gstore Genv e2 (TList TBool) ->
-        type_of Gstore Genv (and_bitmaps e1 e2) (TList TBool).
+    Lemma filter_to_bitmap_lookup_head_sound : forall is_tbl_ty' aux_ty aux_wf,
+        aux_ty_for_idx pk_idx_tag pk_idx_ty aux_ty ->
+        aux_ty_for_idx bm_tag bitmap_ty aux_ty ->
+        (forall t, is_tbl_ty' t = true -> is_pk_tbl_ty t = true /\ is_bitmap_tbl_ty t = true) ->
+        (forall (v : value), aux_wf v -> aux_wf_for_idx pk_idx_tag pk_idx_wf v /\ aux_wf_for_idx bm_tag bitmap_wf v) ->
+        expr_aug_transf_sound is_tbl_ty' aux_ty aux_wf (filter_to_bitmap_lookup_head x b acc).
     Proof.
-      clear H_NoDup.
-      intros. econstructor; eauto.
-      repeat econstructor; try now (rewrite_map_get_put_goal; auto).
-      destruct_get_put_strings; auto.
-    Qed.
-
-    Lemma and_filter_to_lookup_head_preserve_ty : forall tl t aux_tl (Gstore : tenv),
-        type_wf t -> is_pk_tbl_ty t = true ->
-        is_bitmap_tbl_ty attr1 t = true ->
-        is_bitmap_tbl_ty attr2 t = true ->
-        map.get Gstore tbl = Some (TRecord tl) ->
-        access_record tl id_tag = Success t ->
-        access_record tl aux_tag = Success (TRecord aux_tl) ->
-        access_record aux_tl pk_idx_tag = Success (pk_idx_ty t) ->
-        access_record aux_tl bm1_tag = Success (bitmap_ty t) ->
-        access_record aux_tl bm2_tag = Success (bitmap_ty t) ->
-        preserve_ty Gstore (and_filter_to_lookup_head).
-    Proof.
-      unfold preserve_ty, is_pk_tbl_ty, is_bitmap_tbl_ty. intros.
-      repeat destruct_match_hyp; try congruence.
-      repeat destruct_subexpr. simpl.
-      case_match; auto. repeat rewrite Bool.andb_true_r in *.
-      repeat rewrite Bool.andb_true_iff in *; intuition idtac.
-      rewrite eqb_eq in *; subst.
-      repeat invert_type_of_clear. repeat invert_type_of_op_clear.
-      repeat rewrite_map_get_put_hyp.
-      repeat (clear_refl; repeat do_injection2).
-      repeat (rewrite_l_to_r; do_injection2).
-      econstructor.
-      1: econstructor.
-      1: apply and_bitmaps_ty; repeat (econstructor; eauto).
-      1:{ lazymatch goal with
-          H: tenv_wf ?G, H': map.get ?G _ = _ |- _ =>
-            apply H in H'
-        end.
-          repeat invert_type_wf.
-          instantiate(1:=[("0", TInt); ("1", TList (TRecord tl1))]).
-          repeat (econstructor; eauto). cbn; intuition discriminate. }
-      1:{ repeat (econstructor; eauto);
-          repeat rewrite_map_get_put_goal; eauto;
-          use_is_NoDup. }
-      cbn; reflexivity.
-    Qed.
-
-    Context (pk_hole pk_tup pk_acc : string).
-    Context (H_NoDup_pk : is_NoDup_opaque [pk_tup; pk_acc]).
-
-    Notation pk_idx_wf := (pk_idx_wf pk_hole pk_tup pk_acc).
-
-    Definition aux_wf_for_idx idx_tag idx_wf (v : value) : Prop :=
-      match v with
-      | VRecord rv =>
-          match access_record rv id_tag with
-          | Success v_id =>
-              match access_record rv aux_tag with
-              | Success (VRecord rv_aux) =>
-                  match access_record rv_aux idx_tag with
-                  | Success v_idx =>
-                      idx_wf v_id v_idx
-                  | _ => False
-                  end
-              | _ => False
-              end
-          | _ => False
-          end
-      | _ => False
-      end.
-
-    Context (bm1_hole bm2_hole : string).
-    Context (bm1_tup bm2_tup : string).
-    Notation bitmap1_wf := (bitmap_wf attr1 str1 bm1_hole bm1_tup).
-    Notation bitmap2_wf := (bitmap_wf attr2 str2 bm2_hole bm2_tup).
-
-    (* ??? TODO: move *)
-    Lemma Forall2_access_record : forall A A' P l l' x (a : A) (a' : A'),
-        Forall2 (fun p p' => fst p = fst p' /\ P (snd p) (snd p')) l l' ->
-        access_record l x = Success a ->
-        access_record l' x = Success a' ->
-        P a a'.
-    Proof.
-      induction 1; cbn; try discriminate; auto.
-      repeat case_match; cbn in *; intuition idtac;
-        repeat (try clear_refl; do_injection); subst; auto;
-        congruence.
-    Qed.
-
-    Ltac use_Forall2_access_record tag :=
+      unfold aux_ty_for_idx, expr_aug_transf_sound; intros.
+      invert_tenv_wf_with_globals.
       lazymatch goal with
-        H: Forall2 _ ?l ?tl, H1: access_record ?l tag = _,
-            H2: access_record ?tl tag = _ |- _ =>
-          pose proof (Forall2_access_record _ _ _ _ _ _ _ _ H H1 H2)
+        H: forall _, is_tbl_ty' _ = _ -> _, H': is_tbl_ty' _ = _ |- _ =>
+        apply H in H' end; destruct_and.
+      specialize (H tbl_ty). specialize (H0 tbl_ty).
+      repeat destruct_match_hyp; intuition idtac.
+      1: eapply filter_to_bitmap_lookup_head_preserve_ty; eauto.
+      1: eapply filter_to_bitmap_lookup_head_preserve_sem; eauto.
+      lazymatch goal with
+        H: locals_wf ?G ?str, H': map.get ?G _ = _ |- _ =>
+          apply H in H'
       end.
-
-    Lemma and_filter_to_lookup_head_preserve_sem : forall (Gstore : tenv) (store : locals) tl t aux_tl,
-        type_wf t -> is_pk_tbl_ty t = true ->
-        is_bitmap_tbl_ty attr1 t = true ->
-        is_bitmap_tbl_ty attr2 t = true ->
-        map.get Gstore tbl = Some (TRecord tl) ->
-        access_record tl id_tag = Success t ->
-        access_record tl aux_tag = Success (TRecord aux_tl) ->
-        access_record aux_tl pk_idx_tag = Success (pk_idx_ty t) ->
-        access_record aux_tl bm1_tag = Success (bitmap_ty t) ->
-        access_record aux_tl bm2_tag = Success (bitmap_ty t) ->
-        match map.get store tbl with
-        | Some v => aux_wf_for_idx pk_idx_tag pk_idx_wf v /\
-                      aux_wf_for_idx bm1_tag bitmap1_wf v /\
-                      aux_wf_for_idx bm2_tag bitmap2_wf v
-        | _ => False
-        end ->
-        preserve_sem Gstore store and_filter_to_lookup_head.
-    Proof.
-      unfold preserve_sem, aux_wf_for_idx; intros.
-      unfold is_pk_tbl_ty, is_bitmap_tbl_ty, pk_idx_ty, bitmap_ty in *.
-      apply_locals_wf store.
-      repeat (destruct_match_hyp; try discriminate; intuition idtac; []).
-
-      invert_type_of_value_clear.
-      use_Forall2_access_record id_tag.
-      use_Forall2_access_record aux_tag.
-      invert_type_of_value_clear.
-      use_Forall2_access_record pk_idx_tag.
-      use_Forall2_access_record bm1_tag.
-      use_Forall2_access_record bm2_tag.
-      repeat destruct_subexpr. unfold and_filter_to_lookup_head.
-      case_match; auto. cbn in * |-.
-      repeat rewrite Bool.andb_true_iff in *; intuition idtac.
-      rewrite eqb_eq in *; subst. repeat clear_refl.
-      unfold use_bitmap, and_bitmaps.
-      cbn [interp_expr interp_binop apply_bool_binop].
-      unfold get_local. rewrite_l_to_r.
-      unfold record_proj. repeat rewrite_l_to_r.
-      repeat invert_type_of_value_clear.
-
-
+      destruct_match_hyp; intuition idtac.
+      all: lazymatch goal with
+             H: holds_for_all_entries _ ?str, H': map.get ?str _ = _ |- _ =>
+               apply H in H'
+           end.
+      all: unfold value_wf_with_globals in *; invert_Forall; intuition idtac.
+      all: lazymatch goal with
+             H: context[?f _ _]|- ?f _ _ _ =>
+               apply H end; auto.
+    Qed.
   End WithMap.
-*)
+End WithTags.
